Define reduction

00.v
@@ -1,4 +1,8 @@
 (*Definition var := nat.*)
+Require Import Coq.Program.Tactics.
+Require Import Coq.Program.Wf.
+Require Import Omega.
+
 Section var.
 Context (var:Set) (deq:var->var->bool).
 Inductive term :=
@@ -13,6 +17,22 @@ Inductive func :=
 | subs : func -> var -> func
 .
 
+Fixpoint lent (t:term) : nat :=
+match t with
+ | atom x => 0
+ | appl x x0 => (max (lent x) (lent x0))+1
+ | lamb x x0 => (lent x0)+2
+ | shft x => (lent x)+1
+end
+.
+
+Fixpoint lenf (f:func) : nat :=
+match f with
+ | varp x x0 => 0
+ | subs x x0 => (lenf x)+1
+end
+.
+
 Fixpoint act (f:func) (t:term) {struct t} : term.
 destruct t as [v|M N|x M|M].
 + destruct f as [y x|F x].
@@ -24,5 +44,53 @@ destruct t as [v|M N|x M|M].
   - exact (shft M).
   - exact (shft (act F M)).
 Show Proof.
-(*Defined.*)
 Abort.
+
+Program Fixpoint act (t : term) (f : func) {measure ((lenf f)+(lent t))} : term :=
+   match t with
+   | atom v =>
+       match f with
+       | varp y x => if deq v x then atom y else shft x
+       | subs F x => if deq v x then atom v else shft (act v F)
+       end
+   | appl M N => appl (act M f) (act N f)
+   | lamb x M => lamb x (act M (subs f x))
+   | shft M =>
+       match f with
+       | varp _ _ => shft M
+       | subs F _ => shft (act M F)
+       end
+   end
+(*with actx (t : term) (f : func) {struct t} :=true*)
+.
+
+Next Obligation.
+simpl. omega.
+Defined.
+Next Obligation.
+simpl.
+Admitted.
+Next Obligation.
+simpl.
+Admitted.
+Next Obligation.
+simpl. omega.
+Defined.
+Next Obligation.
+simpl.
+omega.
+Defined.
+End var.
+(*
+Context (x y:var) (H: deq x y = false).
+Compute (act (lamb x (lamb y x)) (varp y x)).
+*)
+Definition x:=0.
+Definition y:=1.
+(*Compute (act (lamb x (lamb y x)) (varp y x)).*)
+(* DO NOT RUN IT:
+Check (lamb nat y (atom _ x)).
+Compute (act _ _ (lamb _ x (lamb _ y (atom _ x))) 
+).
+(varp nat y x)
+*)
